theories/Semantics/IMP/AxiomaticCompleteness.v
@@ -136,12 +136,6 @@ Proof.
       by lia.
 Qed.
 
-Definition beta_z_helper (x : nat) (y : Z) : Prop :=
-    exists (z : nat),
-      (x = 2 * z -> y = Z.of_nat z)
-        /\
-      (x = 2 * z + 1 -> y = (- Z.of_nat z)%Z).
-
 Definition eb_beta_z_helper (x y : EAExp L V) (z := fresh (alog_vars x ∪ alog_vars y)) : EBExp L V :=
     EAnd (EALe (EAVal 0) x)
     (eb_exists z
@@ -179,9 +173,6 @@ Proof.
       split; [by lia |].
       by exists (Z.of_nat z); lia.
 Qed.
-
-Definition beta_z (n m j : nat) (y : Z) : Prop :=
-    beta_z_helper (beta_fn n m j) y.
 
 Definition eb_beta_z (n m j y : EAExp L V)
     (x := fresh (alog_vars n ∪ alog_vars m ∪ alog_vars j ∪ alog_vars y)) : EBExp L V :=
@@ -226,7 +217,6 @@ Qed.
 
 End sec_goedel.
 
-(*
 Section sec_weakest_precondition.
 
 Definition ws (c : Cmd L) (B : EBExp L V) (I : State V) : Ensemble (State L) :=
@@ -240,12 +230,163 @@ Lemma ws_weakest :
   sem I A ⊆ ws c B I.
 Proof. done. Qed.
 
+Definition WeakestPrecondition (A : EBExp L V) (c : Cmd L) (B : EBExp L V) : Prop :=
+    forall (I : State V), sem I A ≡ ws c B I.
+
+Section sec_wp_oracle.
+
+Context
+    (wp : forall  (c : Cmd L) (B : EBExp L V), {A : EBExp L V | WeakestPrecondition A c B}).
+
+Lemma wp_oracle_weakest : forall (A : EBExp L V) (c : Cmd L) (B : EBExp L V),
+    ht_sat (ht A c B) -> sat (eb_impl A (` (wp c B))).
+Proof.
+    intros * Hht sigma I.
+    specialize (Hht I).
+    rewrite ws_weakest in Hht.
+    destruct (wp c B) as [A' HA']; rewrite classical_satsi_impl; intro HA.
+    by apply HA', Hht.
+Qed.
+
+Lemma wp_oracle_skip : forall (B : EBExp L V),
+    sat (eb_iff (` (wp Skip B))  B).
+Proof.
+    intros; destruct wp as [A Hwp].
+    intros sigma I; apply satsi_iff; split.
+    - by intro HA; apply Hwp in HA; apply HA.
+    - intro HB; apply Hwp.
+      by intro sigma'; inversion 1; subst.
+Qed.
+
+Lemma wp_oracle_asgn : forall (B : EBExp L V) (l : L) (a : AExp L),
+    sat (eb_iff (` (wp (Asgn l a) B)) (bsubst B subst0 (mk_subst [(l, a)]))).
+Proof.
+    intros; destruct wp as [A Hwp].
+    intros sigma I; apply satsi_iff; split.
+    - intro HA; apply Hwp in HA.
+      by apply satsi_subst_loc, HA; constructor.
+    - intro HB; apply Hwp.
+      intro sigma'; inversion 1; subst.
+      by apply satsi_subst_loc.
+Qed.
+
+Lemma wp_oracle_seq : forall (B : EBExp L V) (c1 c2 : Cmd L),
+    sat (eb_iff (` (wp (Seq c1 c2) B)) (` (wp c1 (` (wp c2 B))))).
+Proof.
+    intros.
+    destruct (wp (Seq c1 c2) B) as [A Hseq].
+    destruct (wp c2 B) as [A2 Hc2]; cbn.
+    destruct (wp c1 A2) as [A1 Hc1]; cbn.
+    intros sigma I; apply satsi_iff; split.
+    - intros HA; apply Hseq in HA.
+      apply Hc1.
+      intros sigma' Hss'.
+      apply Hc2.
+      intros sigma'' Hss''.
+      by apply HA; econstructor.
+    - intros HA1; apply Hseq.
+      intros sigma' Hss'.
+      apply elem_of_fwd_relation_composition in Hss' as (sigma'' & Hss'' & Hss''').
+      eapply Hc2; [| done].
+      by eapply Hc1.
+Qed.
+
+Lemma wp_oracle_if : forall (B : EBExp L V) (b : BExp L) (c1 c2 : Cmd L),
+    sat (eb_iff (` (wp (If b c1 c2) B)) (EOr (EAnd b (` (wp c1 B))) (EAnd (ENot b) (` (wp c2 B))))).
+Proof.
+    intros.
+    destruct (wp (If b c1 c2) B) as [A Hif].
+    destruct (wp c1 B) as [A1 Hc1]; cbn.
+    destruct (wp c2 B) as [A2 Hc2]; cbn.
+    intros sigma I.
+    rewrite satsi_iff, satsi_or, !satsi_and, satsi_not; split.
+    - intros HA; apply Hif in HA.
+      rewrite satsi_eval.
+      destruct (decide (denotb b sigma = true)); [left | right]; (split; [done |]).
+      + apply Hc1; intros sigma' Hss'; apply HA.
+        by apply elem_of_relation_selector; left.
+      + apply Hc2; intros sigma' Hss'; apply HA.
+        apply elem_of_relation_selector; right; split; [| done].
+        by destruct denotb.
+    - rewrite satsi_eval. intros [[Hb HA1] | [Hnb HA2]]; apply Hif;
+        intros sigma' Hss'; apply elem_of_relation_selector in Hss' as [[]|[]].
+      + by eapply Hc1.
+      + by congruence.
+      + by congruence.
+      + by eapply Hc2.
+Qed.
+
+Lemma wp_oracle_while_inv : forall (B : EBExp L V) (b : BExp L) (c : Cmd L),
+    ht_sat (ht (EAnd (` (wp (While b c) B)) b) c (` (wp (While b c) B))).
+Proof.
+    intros.
+    destruct (wp (While b c) B) as [A Hwhile]; cbn.
+    intros I sigma Hpre sigma' Hss'; cbn in *.
+    apply Hwhile; intros sigma'' Hss''.
+    apply satsi_and in Hpre as [HA Hb].
+    apply satsi_eval in Hb.
+    apply Hwhile with sigma; [done |].
+    apply knaster_tarski_lfp_fix; [by typeclasses eauto |].
+    apply elem_of_while_step; right.
+    split; [done |].
+    by exists sigma'.
+Qed.
+
+Lemma wp_oracle_while_exit : forall (B : EBExp L V) (b : BExp L) (c : Cmd L),
+    sat (eb_impl (EAnd (` (wp (While b c) B)) (ENot b)) B).
+Proof.
+    intros.
+    destruct (wp (While b c) B) as [A Hwhile]; intros sigma I; cbn.
+    rewrite classical_satsi_impl, satsi_and, satsi_not, satsi_eval.
+    intros [HA Hb].
+    apply Hwhile in HA; apply HA.
+    apply knaster_tarski_lfp_fix; [by typeclasses eauto |].
+    by right; [destruct denotb | constructor].
+Qed.
+
+Lemma wp_oracle_ht_ded :
+    forall (c : Cmd L) (B : EBExp L V), ht_ded (ht (` (wp c B)) c B).
+Proof.
+    induction c; intros B; [eapply ht_cons;
+        [| econstructor | by intros sigma I; apply classical_satsi_impl]..|].
+    - by apply sat_iff_lr, wp_oracle_skip.
+    - by apply sat_iff_lr, wp_oracle_asgn.
+    - by apply sat_iff_lr, wp_oracle_seq.
+    - by apply IHc1.
+    - by apply IHc2.
+    - by apply sat_iff_lr, wp_oracle_if.
+    - eapply ht_cons; cycle 2; [by intros sigma I; apply classical_satsi_impl | | by apply IHc1].
+      intros I sigma.
+      rewrite classical_satsi_impl, satsi_and, satsi_or, !satsi_and, satsi_not.
+      by tauto.
+    - eapply ht_cons; cycle 2; [by intros sigma I; apply classical_satsi_impl | | by apply IHc2].
+      intros I sigma.
+      rewrite classical_satsi_impl, satsi_and, satsi_or, !satsi_and, satsi_not.
+      by tauto.
+    - eapply ht_cons; cycle 1;
+        [constructor | by apply wp_oracle_while_exit | by intros ? ?; apply classical_satsi_impl].
+      eapply ht_cons; cycle 2; [by intros ? ?; apply classical_satsi_impl | | apply IHc].
+      by apply wp_oracle_weakest, wp_oracle_while_inv.
+Qed.
+
+Lemma wp_oracle_completeness :
+    forall (A : EBExp L V) (c : Cmd L) (B : EBExp L V),
+    ht_sat (ht A c B) -> ht_ded (ht A c B).
+Proof.
+    intros * Hht.
+    eapply ht_cons; cycle 2;
+      [by intros ? ?; apply classical_satsi_impl | | by apply wp_oracle_ht_ded].
+    by apply wp_oracle_weakest.
+Qed.
+
+End sec_wp_oracle.
+
 Section sec_wp_while.
 
 Context
     (b : BExp L) (c : Cmd L) (w : Cmd L := While b c)
     (B : EBExp L V)
-    (relevant_vars : list L := elements (bloc_vars B ∪ cloc_vars w))
+    (relevant_vars : list L := elements (bloc_vars B ∪ cloc_vars (V := V) w))
     .
 
 Inductive WhileOpenSequence : State L -> list (State L) -> State L -> Prop :=
@@ -348,5 +489,4 @@ match c with
 end.
 
 End sec_weakest_precondition.
-*)
 End sec_axiomatic_completeness.
